#127 monofun for ndaToDo, #162 basics for knasterTarski

automat/ndAutomaton.thy
@@ -2,7 +2,7 @@
 
 theory ndAutomaton
 
-imports spec.SPS SpsStep NDA_functions
+imports spec.SPS SpsStep KnasterTarski
 
 
 begin
@@ -16,43 +16,57 @@ fun ndaWell::"((('state \<times>(channel \<rightharpoonup> 'm)) \<Rightarrow> ((
 (* FYI: Non-deterministic version *)
 cpodef ('state::type, 'm::message) ndAutomaton = 
   "{f::(('state \<times>(channel \<rightharpoonup> 'm)) \<Rightarrow> (('state \<times> 'm SB) set rev)) \<times> ('state \<times> 'm SB) set rev \<times> channel set discr \<times> channel set discr. ndaWell f}"
-  sorry
+    sorry
 
 setup_lifting type_definition_ndAutomaton
 
+(* ToDo Move this somewhere else. eg prelude *)
+setup_lifting type_definition_cfun
 
 
-definition ndaTransition :: "('s, 'm::message) ndAutomaton \<rightarrow> (('s \<times>(channel \<rightharpoonup> 'm)) \<Rightarrow> (('s \<times> 'm SB) set rev))" where
-"ndaTransition \<equiv> \<Lambda> nda. fst (Rep_ndAutomaton nda)"
+lemma nda_rep_cont[simp]: "cont Rep_ndAutomaton"
+  by (simp add: cont_Rep_ndAutomaton)
 
-definition ndaInitialState :: "('s, 'm::message) ndAutomaton \<rightarrow> ('s \<times> 'm SB) set rev" where
-"ndaInitialState = (\<Lambda> nda. fst (snd (Rep_ndAutomaton nda)))"
 
-definition ndaDom :: "('s, 'm::message) ndAutomaton \<rightarrow> channel set" where
-"ndaDom = (\<Lambda> nda. undiscr(fst (snd (snd (Rep_ndAutomaton nda)))))"
 
-definition ndaRan :: "('s, 'm::message) ndAutomaton \<rightarrow> channel set" where
-"ndaRan =  (\<Lambda> nda. undiscr(snd (snd (snd (Rep_ndAutomaton nda)))))" 
 
-(* ToDo *)
-(* Very Very similar to helper over automaton *)
-thm da_helper_def
+    section \<open>Definitions\<close>
 
-  (* nondeterministic... but is it cont in h ? *)
-definition ndaToDo:: "channel set \<Rightarrow> channel set \<Rightarrow> ('s \<times> 'm::message SB) set rev \<Rightarrow> ('s \<Rightarrow> 'm SPS) \<rightarrow> 'm SPS" where
-"ndaToDo In Out S \<equiv> \<Lambda> h. uspecFlatten In Out 
+
+lift_definition ndaTransition :: "('s, 'm::message) ndAutomaton \<rightarrow> (('s \<times>(channel \<rightharpoonup> 'm)) \<Rightarrow> (('s \<times> 'm SB) set rev))" is
+"\<lambda>nda. fst (Rep_ndAutomaton nda)"
+  by (simp add: cfun_def)
+
+lift_definition ndaInitialState :: "('s, 'm::message) ndAutomaton \<rightarrow> ('s \<times> 'm SB) set rev" is
+"(\<lambda> nda. fst (snd (Rep_ndAutomaton nda)))"
+  by (simp add: cfun_def)
+
+lift_definition ndaDom :: "('s, 'm::message) ndAutomaton \<rightarrow> channel set" is
+"(\<lambda> nda. undiscr(fst (snd (snd (Rep_ndAutomaton nda)))))"
+  apply (simp add: cfun_def)
+  by (smt Cont.contI2 below_ndAutomaton_def discrete_cpo is_ub_thelub monofunI po_eq_conv snd_monofun)
+
+lift_definition ndaRan :: "('s, 'm::message) ndAutomaton \<rightarrow> channel set" is
+"(\<lambda> nda. undiscr(snd (snd (snd (Rep_ndAutomaton nda)))))" 
+  apply (simp add: cfun_def)
+  by (smt Cont.contI2 below_ndAutomaton_def discrete_cpo is_ub_thelub monofunI po_eq_conv snd_monofun)
+
+
+  (* Only monofun, not cont *)
+definition ndaToDo:: "channel set \<Rightarrow> channel set \<Rightarrow> ('s \<times> 'm::message SB) set rev \<Rightarrow> ('s \<Rightarrow> 'm SPS) \<Rightarrow> 'm SPS" where
+"ndaToDo In Out S \<equiv> \<lambda> h. uspecFlatten In Out 
                 (setrevImage (\<lambda>(state, sb). spsConcOut sb\<cdot>(h state)) S)"
 
-(* Goals *)
-lemma (* assumes "\<And>s c. s\<in>((inv Rev) S) \<Longrightarrow> c\<in>ubDom\<cdot>(snd s) \<Longrightarrow> # ((snd s) . c) < \<infinity>" *)
-  shows  "monofun(\<lambda> h. uspecFlatten In Out (setrevImage (\<lambda>(state, sb). spsConcOut sb\<cdot>(h state)) S))"
-  apply(rule monofunI)
-  oops
+lemma ndatodo_monofun: "monofun (ndaToDo In Out S)" (is "monofun ?f")
+proof (rule monofunI)
+  fix x y :: "'a \<Rightarrow> 'b SPS"
+  assume "x \<sqsubseteq> y"
+  hence h: "(\<lambda>(state, sb). spsConcOut sb\<cdot>(x state)) \<sqsubseteq> (\<lambda>(state, sb). spsConcOut sb\<cdot>(y state))"
+    by (simp add: below_fun_def cont_pref_eq1I) 
+  thus "?f x \<sqsubseteq> ?f y" by (metis (no_types) h monofun_def ndaToDo_def uspecflatten_image_monofun)
+ qed
 
-lemma "cont(\<lambda> h. uspecFlatten In Out (setrevImage (\<lambda>(state, sb). spsConcOut sb\<cdot>(h state)) S))"
-  oops
-
-lemma "monofun (\<lambda> S. uspecFlatten In Out (setrevImage (\<lambda>(state, sb). spsConcOut sb\<cdot>(some_h state)) S))"
+lemma ndatodo_monofun2: "monofun (\<lambda> S. uspecFlatten In Out (setrevImage (\<lambda>(state, sb). spsConcOut sb\<cdot>(some_h state)) S))"
 proof -
   have b0:  "monofun (\<lambda> S. (setrevImage (\<lambda>(state, sb). spsConcOut sb\<cdot>(some_h state)) S))"
     by (simp add: image_mono_rev monofunE)
@@ -62,9 +76,13 @@ qed
 
 
 
-definition ndaHelper2:: "'s \<Rightarrow> (('s \<times>'e) \<Rightarrow> ('s \<times> 'm::message SB) set rev) \<Rightarrow> ('s \<Rightarrow> 'm SPS) \<rightarrow> ('e \<Rightarrow> 'm SPS)" where
-"ndaHelper2 s transition \<equiv> \<Lambda> h. (\<lambda>e. ndaToDo undefined undefined (transition (s,e))\<cdot>h)"
+definition ndaHelper2:: "channel set \<Rightarrow> channel set \<Rightarrow> 's \<Rightarrow> (('s \<times>'e) \<Rightarrow> ('s \<times> 'm::message SB) set rev) \<Rightarrow> ('s \<Rightarrow> 'm SPS) \<Rightarrow> ('e \<Rightarrow> 'm SPS)" where
+"ndaHelper2 In Out s transition \<equiv> \<lambda> h. (\<lambda>e. ndaToDo In Out (transition (s,e)) h)"
 
+
+lemma ndaHelper2_monofun: "monofun (ndaHelper2 In Out s transition)"
+  unfolding ndaHelper2_def
+  by (metis (mono_tags, lifting) mono2mono_lambda monofun_def ndaToDo_def ndatodo_monofun)
 
 
 (* delete first input element. This is here because "spfStep" does not call "sbRt" and the
@@ -76,21 +94,28 @@ lemma "cont (\<lambda> h. (\<lambda> s. spsRtIn\<cdot>(h s)))"
   by simp
 
 
+definition nda_h_inner::"('s::type, 'm::message) ndAutomaton \<Rightarrow> ('s \<Rightarrow> 'm SPS) \<Rightarrow> ('s \<Rightarrow> 'm SPS)" where
+"nda_h_inner nda h \<equiv>  let dom = (ndaDom\<cdot>nda);
+                          ran = (ndaRan\<cdot>nda) in 
+     (\<lambda>s. spsStep dom ran\<cdot>(ndaAnotherHelper\<cdot>(ndaHelper2 dom ran s (ndaTransition\<cdot>nda) h)))"
+
+lemma nda_h_inner_monofun: "monofun (nda_h_inner nda)"
+  unfolding nda_h_inner_def
+  apply(simp only: Let_def)
+  apply(rule monofunI)
+  by (simp add: fun_belowI monofunE monofun_Rep_cfun2 ndaHelper2_monofun)
+
 
 (* Similar to Rum96 *)
 definition nda_h :: "('s::type, 'm::message) ndAutomaton \<Rightarrow> ('s \<Rightarrow> 'm SPS)" where
-"nda_h nda \<equiv> let dom = (ndaDom\<cdot>nda);
-                 ran = (ndaRan\<cdot>nda) in 
-  uspecStateFix dom ran\<cdot>(\<Lambda> h. (\<lambda>s. spsStep dom ran\<cdot>(ndaAnotherHelper\<cdot>(ndaHelper2 s (ndaTransition\<cdot>nda)\<cdot>h))))"
+"nda_h nda \<equiv> lfp (nda_h_inner nda)"
 
+lemma nda_h_fixpoint: "nda_h nda = nda_h_inner nda (nda_h nda)"
+  by (simp add: lfp_condition nda_h_def nda_h_inner_monofun)
 
 
 definition nda_H :: "('s, 'm::message) ndAutomaton \<Rightarrow> 'm SPS" where
-"nda_H nda \<equiv> ndaToDo (ndaDom\<cdot>nda)(ndaRan\<cdot>nda) (ndaInitialState\<cdot>nda)\<cdot>(nda_h nda)" 
-
-
-lemma nda_rep_cont[simp]: "cont Rep_ndAutomaton"
-  by (simp add: cont_Rep_ndAutomaton)
+"nda_H nda \<equiv> ndaToDo (ndaDom\<cdot>nda)(ndaRan\<cdot>nda) (ndaInitialState\<cdot>nda) (nda_h nda)" 
 
 
 lemma "cont (\<lambda>nda. fst (Rep_ndAutomaton nda))"
