automat/KnasterTarski.thy
@@ -1,0 +1,30 @@
+(* Dummy for KnasterTarski proof over cpo/pcpo *)
+
+theory KnasterTarski
+
+imports HOLCF
+
+begin
+
+(* This is going to be problematic, we cannot use pcpo (because uspec is no pcpo) *)
+default_sort cpo
+
+(* ToDo: add LEAST condition *)
+definition lfp:: "('a \<Rightarrow> 'a) \<Rightarrow> 'a" where
+"lfp f = (SOME x. f x = x)"
+
+lemma knaster_tarski: fixes f :: "'a \<Rightarrow>'a"
+  assumes "monofun f"
+  obtains x where "f x = x"
+  sorry
+
+lemma lfp_condition: assumes "monofun f"
+  shows "f (lfp f) = lfp f"
+  apply(simp add: lfp_def)
+  by (meson assms knaster_tarski someI)
+
+(* We are going to use this for refinement. Does not hold like this, the input might not be monofun *)
+lemma lfp_monofun: "monofun lfp"
+  oops
+
+end
